Generalized nametags, term typing judgement

Isotope/Syntax/NamedList/Ctx.lean
@@ -2,15 +2,15 @@ import Isotope.Syntax.Ty
 
 namespace NamedList
 
-structure Var (T: Type u) extends Transparency where
-  name: String
-  ty: T
+structure Var (N: Type u) (T: Type v) extends Transparency where
+  name: N
+  ty: Ty T
 
-instance Var.instHasLin {T} [HasLin T]: HasLin (Var T) where
+instance Var.instHasLin {N: Type u} {T: Type v} [HasLin T]: HasLin (Var N T) where
   aff v := v.aff && HasLin.aff v.ty
   rel v := v.rel && HasLin.rel v.ty
 
-instance Var.instPartialOrder {T}: PartialOrder (Var T) where
+instance Var.instPartialOrder {N: Type u} {T: Type v}: PartialOrder (Var N T) where
   le l r := l.name = r.name ∧ l.ty = r.ty ∧ l.toTransparency ≤ r.toTransparency
   le_refl := by simp [le_refl]
   le_trans _ _ _
@@ -19,14 +19,14 @@ instance Var.instPartialOrder {T}: PartialOrder (Var T) where
   le_antisymm x x' H H'
     := mk.injEq _ _ _ _ _ _ ▸ ⟨le_antisymm H.2.2 H'.2.2, H.1, H.2.1⟩
 
-theorem Var.le.aff {T} [HasLin T] {l r: Var T}
+theorem Var.le.aff {N: Type u} {T: Type v} [HasLin T] {l r: Var N T}
   : l ≤ r → HasLin.aff l → HasLin.aff r
   | ⟨He, Ht⟩ => by
     simp only [HasLin.aff, He, Bool.and_eq_true, and_imp]
     intro H H';
     exact ⟨Ht.2.1 H, Ht.1 ▸ H'⟩
 
-theorem Var.le.rel {T} [HasLin T] {l r: Var T}
+theorem Var.le.rel {N: Type u} {T: Type v} [HasLin T] {l r: Var N T}
   : l ≤ r → HasLin.rel l → HasLin.rel r
   | ⟨He, Ht⟩ => by
     simp only [HasLin.rel, He, Bool.and_eq_true, and_imp]
@@ -37,27 +37,31 @@ theorem Var.le.rel {T} [HasLin T] {l r: Var T}
 --TODO: contexts as finite functions Name -> Var? could be !FUN!
 --Can be equipped with a separate "domain"?
 --In this case can define separation-style judgements on domains...
-abbrev Ctx (T: Type u) := List (Var T)
+abbrev Ctx (N: Type u) (T: Type v) := List (Var N T)
 
-inductive Ctx.name {T: Type u}: Ctx T -> String -> Prop
-  | head (q n A) (Γ: Ctx T): Ctx.name (⟨q, n, A⟩::Γ) n
+inductive Ctx.name {N: Type u} {T: Type v}: Ctx N T -> N -> Type (max u v)
+  | head (q n A) (Γ: Ctx N T): Ctx.name (⟨q, n, A⟩::Γ) n
   | tail {m Γ} v: Ctx.name Γ m -> Ctx.name (v::Γ) m
 
-instance Ctx.instHasLin {T: Type u} [HasLin T]: HasLin (Ctx T) where
+instance Ctx.instHasLin {N: Type u} {T: Type v} [HasLin T]
+  : HasLin (Ctx N T) where
   aff Γ := Γ.all HasLin.aff
   rel Γ := Γ.all HasLin.rel
 
-inductive Ctx.subctx {T: Type u} [HasLin T]: Ctx T -> Ctx T -> Type u
+inductive Ctx.subctx {N: Type u} {T: Type v} [HasLin T]
+  : Ctx N T -> Ctx N T -> Type (max u v)
   | nil: subctx [] []
-  | cons {Γ Δ} {v l: Var T}: l ≤ v -> subctx Γ Δ -> subctx (v::Γ) (l::Δ)
-  | discard {Γ Δ} (v: Var T): subctx Γ Δ -> subctx (v::Γ) Δ
+  | cons {Γ Δ} {v l: Var N T}: l ≤ v -> subctx Γ Δ -> subctx (v::Γ) (l::Δ)
+  | discard {Γ Δ} (v: Var N T): subctx Γ Δ -> subctx (v::Γ) Δ
 
-def Ctx.is_subctx {T: Type u} [HasLin T] {Γ Δ: Ctx T} := Nonempty (Γ.subctx Δ)
+def Ctx.is_subctx {N: Type u} {T: Type v} [HasLin T] {Γ Δ: Ctx N T}: Prop
+  := Nonempty (Γ.subctx Δ)
 
 --TODO: all subcontexts are unique if and only if all variable names are unique
 --TODO: think of how this could be used to define nameless SSA...
 
-inductive Ctx.split {T: Type u} [HasLin T]: Ctx T → Ctx T → Ctx T → Type u
+inductive Ctx.split {N: Type u} {T: Type v} [HasLin T]
+  : Ctx N T → Ctx N T → Ctx N T → Type (max u v)
   | nil: split [] [] []
   | left {Γ Δ Ξ} {v l}:  l ≤ v → split Γ Δ Ξ → split (v::Γ) (l::Δ) Ξ
   | right {Γ Δ Ξ} {v r}: r ≤ v → split Γ Δ Ξ → split (v::Γ) Δ (r::Ξ)
@@ -65,32 +69,33 @@ inductive Ctx.split {T: Type u} [HasLin T]: Ctx T → Ctx T → Ctx T → Type u
   | dup {Γ Δ Ξ} {v l r}: HasLin.rel v → l ≤ v → r ≤ v → split Γ Δ Ξ
     → split (v::Γ) (l::Δ) (r::Ξ)
 
-def Ctx.split.subctx_left {T: Type u} [HasLin T] {Γ Δ Ξ: Ctx T}
+def Ctx.split.subctx_left {N: Type u} {T: Type v} [HasLin T] {Γ Δ Ξ: Ctx N T}
   : Γ.split Δ Ξ -> Γ.subctx Δ
   | nil => subctx.nil
   | right _ H | discard _ H => subctx.discard _ (subctx_left H)
   | left Hl H | dup _ Hl _ H => subctx.cons Hl (subctx_left H)
 
-def Ctx.split.subctx_right {T: Type u} [HasLin T] {Γ Δ Ξ: Ctx T}
+def Ctx.split.subctx_right {N: Type u} {T: Type v}[HasLin T] {Γ Δ Ξ: Ctx N T}
   : Γ.split Δ Ξ -> Γ.subctx Ξ
   | nil => subctx.nil
   | left _ H | discard _ H => subctx.discard _ (subctx_right H)
   | right Hr H | dup _ _ Hr H => subctx.cons Hr (subctx_right H)
 
 @[match_pattern]
-def Ctx.split.sleft {T: Type u} [HasLin T] {Γ Δ Ξ: Ctx T}
-  (v: Var T): split Γ Δ Ξ -> split (v::Γ) (v::Δ) Ξ
+def Ctx.split.sleft {N: Type u} {T: Type v}[HasLin T] {Γ Δ Ξ: Ctx N T}
+  (v: Var N T): split Γ Δ Ξ -> split (v::Γ) (v::Δ) Ξ
   := left (le_refl v)
 @[match_pattern]
-def Ctx.split.sright {T: Type u} [HasLin T] {Γ Δ Ξ: Ctx T}
-  (v: Var T): split Γ Δ Ξ -> split (v::Γ) Δ (v::Ξ)
+def Ctx.split.sright {N: Type u} {T: Type v}[HasLin T] {Γ Δ Ξ: Ctx N T}
+  (v: Var N T): split Γ Δ Ξ -> split (v::Γ) Δ (v::Ξ)
   := right (le_refl v)
 @[match_pattern]
-def Ctx.split.sdup {T: Type u} [HasLin T] {Γ Δ Ξ: Ctx T}
+def Ctx.split.sdup {N: Type u} {T: Type v}[HasLin T] {Γ Δ Ξ: Ctx N T}
   {v} (Hv: HasLin.rel v): split Γ Δ Ξ -> split (v::Γ) (v::Δ) (v::Ξ)
   := dup Hv (le_refl v) (le_refl v)
 
-inductive Ctx.ssplit {T: Type u} [HasLin T]: Ctx T → Ctx T → Ctx T → Type u
+inductive Ctx.ssplit {N: Type u} {T: Type v} [HasLin T]
+  : Ctx N T → Ctx N T → Ctx N T → Type (max u v)
   | nil: ssplit [] [] []
   | left {Γ Δ Ξ} {v l}:  l ≤ v → ssplit Γ Δ Ξ → ssplit (v::Γ) (l::Δ) Ξ
   | right {Γ Δ Ξ} {v r}: r ≤ v → ssplit Γ Δ Ξ → ssplit (v::Γ) Δ (r::Ξ)
@@ -98,26 +103,26 @@ inductive Ctx.ssplit {T: Type u} [HasLin T]: Ctx T → Ctx T → Ctx T → Type 
     → ssplit (v::Γ) (l::Δ) (r::Ξ)
 
 @[match_pattern]
-def Ctx.ssplit.sleft {T: Type u} [HasLin T] {Γ Δ Ξ: Ctx T}
-  (v: Var T): ssplit Γ Δ Ξ -> ssplit (v::Γ) (v::Δ) Ξ
+def Ctx.ssplit.sleft {N: Type u} {T: Type v} [HasLin T] {Γ Δ Ξ: Ctx N T}
+  (v: Var N T): ssplit Γ Δ Ξ -> ssplit (v::Γ) (v::Δ) Ξ
   := left (le_refl v)
 @[match_pattern]
-def Ctx.ssplit.sright {T: Type u} [HasLin T] {Γ Δ Ξ: Ctx T}
-  (v: Var T): ssplit Γ Δ Ξ -> ssplit (v::Γ) Δ (v::Ξ)
+def Ctx.ssplit.sright {N: Type u} {T: Type v} [HasLin T] {Γ Δ Ξ: Ctx N T}
+  (v: Var N T): ssplit Γ Δ Ξ -> ssplit (v::Γ) Δ (v::Ξ)
   := right (le_refl v)
 @[match_pattern]
-def Ctx.ssplit.sdup {T: Type u} [HasLin T] {Γ Δ Ξ: Ctx T}
+def Ctx.ssplit.sdup {N: Type u} {T: Type v} [HasLin T] {Γ Δ Ξ: Ctx N T}
   {v} (Hv: HasLin.rel v): ssplit Γ Δ Ξ -> ssplit (v::Γ) (v::Δ) (v::Ξ)
   := dup Hv (le_refl v) (le_refl v)
 
-def Ctx.ssplit.toSplit {T: Type u} [HasLin T] {Γ Δ Ξ: Ctx T}
+def Ctx.ssplit.toSplit {N: Type u} {T: Type v} [HasLin T] {Γ Δ Ξ: Ctx N T}
   : ssplit Γ Δ Ξ → split Γ Δ Ξ
   | nil => split.nil
   | left Hl H => split.left Hl (ssplit.toSplit H)
   | right Hr H => split.right Hr (ssplit.toSplit H)
   | dup Hrel Hl Hr H => split.dup Hrel Hl Hr (ssplit.toSplit H)
 
-def Ctx.split.swap {T: Type u} [HasLin T] {Γ Δ Ξ: Ctx T}
+def Ctx.split.swap {N: Type u} {T: Type v} [HasLin T] {Γ Δ Ξ: Ctx N T}
   : split Γ Δ Ξ -> split Γ Ξ Δ
   | nil => nil
   | left Hl H => right Hl (swap H)
@@ -126,50 +131,51 @@ def Ctx.split.swap {T: Type u} [HasLin T] {Γ Δ Ξ: Ctx T}
   | dup H Hl Hr HΓ
     => dup H Hr Hl (swap HΓ)
 
-def Ctx.ssplit.swap {T: Type u} [HasLin T] {Γ Δ Ξ: Ctx T}
+def Ctx.ssplit.swap {N: Type u} {T: Type v} [HasLin T] {Γ Δ Ξ: Ctx N T}
   : ssplit Γ Δ Ξ -> ssplit Γ Ξ Δ
   | nil => nil
   | left Hl H => right Hl (swap H)
   | right Hr H => left Hr (swap H)
   | dup Hrel Hl Hr H => dup Hrel Hr Hl (swap H)
 
-def Ctx.ssplit.swap_toSplit {T: Type u} [HasLin T] {Γ Δ Ξ: Ctx T}
+def Ctx.ssplit.swap_toSplit {N: Type u} {T: Type v} [HasLin T] {Γ Δ Ξ: Ctx N T}
   : (H: ssplit Γ Δ Ξ) -> H.swap.toSplit = H.toSplit.swap
   | nil => rfl
   | left _ H => congrArg _ (swap_toSplit H)
   | right _ H => congrArg _ (swap_toSplit H)
   | dup _ _ _ H => congrArg _ (swap_toSplit H)
 
-def Ctx.split.swap_idem {T: Type u} [HasLin T] {Γ Δ Ξ: Ctx T}
-  : Function.LeftInverse (@swap T _ Γ Δ Ξ) (@swap T _ Γ Ξ Δ)
+def Ctx.split.swap_idem {N: Type u} {T: Type v} [HasLin T] {Γ Δ Ξ: Ctx N T}
+  : Function.LeftInverse (@swap N T _ Γ Δ Ξ) (@swap N T _ Γ Ξ Δ)
   | nil => rfl
   | left _ HΓ => by simp [swap, swap_idem HΓ]
   | right _ HΓ => by simp [swap, swap_idem HΓ]
   | discard _ HΓ => by simp [swap, swap_idem HΓ]
   | dup _ _ _ HΓ => by simp [swap, swap_idem HΓ]
 
-def Ctx.ssplit.swap_idem {T: Type u} [HasLin T] {Γ Δ Ξ: Ctx T}
-  : Function.LeftInverse (@swap T _ Γ Δ Ξ) (@swap T _ Γ Ξ Δ)
+def Ctx.ssplit.swap_idem {N: Type u} {T: Type v} [HasLin T] {Γ Δ Ξ: Ctx N T}
+  : Function.LeftInverse (@swap N T _ Γ Δ Ξ) (@swap N T _ Γ Ξ Δ)
   | nil => rfl
   | left _ H => by simp [swap, swap_idem H]
   | right _ H => by simp [swap, swap_idem H]
   | dup _ _ _ H => by simp [swap, swap_idem H]
 
-def Ctx.split.swap_equiv {T: Type u} [HasLin T] (Γ Δ Ξ: Ctx T)
+def Ctx.split.swap_equiv {N: Type u} {T: Type v} [HasLin T] (Γ Δ Ξ: Ctx N T)
   : Equiv (split Γ Δ Ξ) (split Γ Ξ Δ) where
   toFun := swap
   invFun := swap
   left_inv := swap_idem
   right_inv := swap_idem
 
-def Ctx.ssplit.swap_equiv {T: Type u} [HasLin T] (Γ Δ Ξ: Ctx T)
+def Ctx.ssplit.swap_equiv {N: Type u} {T: Type v} [HasLin T] (Γ Δ Ξ: Ctx N T)
   : Equiv (ssplit Γ Δ Ξ) (ssplit Γ Ξ Δ) where
   toFun := swap
   invFun := swap
   left_inv := swap_idem
   right_inv := swap_idem
 
-theorem Ctx.split.left_length_decreasing {T: Type u} [HasLin T] {Γ Δ Ξ: Ctx T}
+theorem Ctx.split.left_length_decreasing {N: Type u} {T: Type v} [HasLin T]
+  {Γ Δ Ξ: Ctx N T}
   : split Γ Δ Ξ -> Δ.length ≤ Γ.length
   | nil => le_refl _
   | left _ HΓ => Nat.succ_le_succ HΓ.left_length_decreasing
@@ -177,57 +183,60 @@ theorem Ctx.split.left_length_decreasing {T: Type u} [HasLin T] {Γ Δ Ξ: Ctx T
   | discard _ HΓ => Nat.le_step HΓ.left_length_decreasing
   | dup _ _ _ HΓ => Nat.succ_le_succ HΓ.left_length_decreasing
 
-theorem Ctx.ssplit.left_length_decreasing {T: Type u} [HasLin T] {Γ Δ Ξ: Ctx T}
-  (H: ssplit Γ Δ Ξ): Δ.length ≤ Γ.length
+theorem Ctx.ssplit.left_length_decreasing {N: Type u} {T: Type v} [HasLin T]
+  {Γ Δ Ξ: Ctx N T} (H: ssplit Γ Δ Ξ): Δ.length ≤ Γ.length
   := H.toSplit.left_length_decreasing
 
-theorem Ctx.split.right_length_decreasing {T: Type u} [HasLin T] {Γ Δ Ξ: Ctx T}
-  (H: split Γ Δ Ξ): Ξ.length ≤ Γ.length
+theorem Ctx.split.right_length_decreasing {N: Type u} {T: Type v} [HasLin T]
+  {Γ Δ Ξ: Ctx N T} (H: split Γ Δ Ξ): Ξ.length ≤ Γ.length
   := H.swap.left_length_decreasing
 
-theorem Ctx.ssplit.right_length_decreasing {T: Type u} [HasLin T] {Γ Δ Ξ: Ctx T}
-  (H: ssplit Γ Δ Ξ): Ξ.length ≤ Γ.length
+theorem Ctx.ssplit.right_length_decreasing {N: Type u} {T: Type v} [HasLin T]
+  {Γ Δ Ξ: Ctx N T} (H: ssplit Γ Δ Ξ): Ξ.length ≤ Γ.length
   := H.toSplit.right_length_decreasing
 
-def Ctx.wk {T: Type u} [HasLin T] (Γ Δ: Ctx T) := Ctx.split Γ Δ []
-def Ctx.var {T: Type u} [HasLin T] (Γ: Ctx T) (x: Var T) := Ctx.wk Γ [x]
+def Ctx.wk {N: Type u} {T: Type v} [HasLin T] (Γ Δ: Ctx N T)
+  := Ctx.split Γ Δ []
+def Ctx.var {N: Type u} {T: Type v} [HasLin T] (Γ: Ctx N T) (x: Var N T)
+  := Ctx.wk Γ [x]
 
 @[match_pattern]
-def Ctx.wk.nil {T: Type u} [HasLin T]: @Ctx.wk T _ [] [] := Ctx.split.nil
+def Ctx.wk.nil {N: Type u} {T: Type v} [HasLin T]: @Ctx.wk N T _ [] []
+  := Ctx.split.nil
 @[match_pattern]
-def Ctx.wk.cons {T: Type u} [HasLin T] {Γ Δ: Ctx T}
-  : {v l: Var T} -> (Hl: l ≤ v) -> Ctx.wk Γ Δ -> Ctx.wk (v::Γ) (l::Δ)
+def Ctx.wk.cons {N: Type u} {T: Type v} [HasLin T] {Γ Δ: Ctx N T}
+  : {v l: Var N T} -> (Hl: l ≤ v) -> Ctx.wk Γ Δ -> Ctx.wk (v::Γ) (l::Δ)
   := Ctx.split.left
   @[match_pattern]
-def Ctx.wk.scons {T: Type u} [HasLin T] {Γ Δ: Ctx T}
-  (v: Var T): Ctx.wk Γ Δ -> Ctx.wk (v::Γ) (v::Δ)
+def Ctx.wk.scons {N: Type u} {T: Type v} [HasLin T] {Γ Δ: Ctx N T}
+  (v: Var N T): Ctx.wk Γ Δ -> Ctx.wk (v::Γ) (v::Δ)
   := Ctx.split.left (le_refl v)
 @[match_pattern]
-def Ctx.wk.discard {T: Type u} [HasLin T] {Γ Δ: Ctx T}
-  : {v: Var T} -> (Ha: HasLin.aff v) -> Ctx.wk Γ Δ -> Ctx.wk (v::Γ) Δ
+def Ctx.wk.discard {N: Type u} {T: Type v} [HasLin T] {Γ Δ: Ctx N T}
+  : {v: Var N T} -> (Ha: HasLin.aff v) -> Ctx.wk Γ Δ -> Ctx.wk (v::Γ) Δ
   := Ctx.split.discard
 
 @[match_pattern]
-def Ctx.var.head {T: Type u} [HasLin T] {Γ: Ctx T}
-  {v v': Var T} (H: v ≥ v') (W: Γ.wk []): Ctx.var (v::Γ) v'
+def Ctx.var.head {N: Type u} {T: Type v} [HasLin T] {Γ: Ctx N T}
+  {v v': Var N T} (H: v ≥ v') (W: Γ.wk []): Ctx.var (v::Γ) v'
   := Ctx.wk.cons H W
 @[match_pattern]
-def Ctx.var.shead {T: Type u} [HasLin T] {Γ: Ctx T}
-  (v: Var T) (W: Γ.wk []): Ctx.var (v::Γ) v
+def Ctx.var.shead {N: Type u} {T: Type v} [HasLin T] {Γ: Ctx N T}
+  (v: Var N T) (W: Γ.wk []): Ctx.var (v::Γ) v
   := Ctx.wk.scons v W
 @[match_pattern]
-def Ctx.var.tail {T: Type u} [HasLin T] {Γ: Ctx T}
-  {v a: Var T} (Ha: HasLin.aff a) (W: Γ.var v): Ctx.var (a::Γ) v
+def Ctx.var.tail {N: Type u} {T: Type v} [HasLin T] {Γ: Ctx N T}
+  {v a: Var N T} (Ha: HasLin.aff a) (W: Γ.var v): Ctx.var (a::Γ) v
   := Ctx.wk.discard Ha W
 
-theorem Ctx.var.name {T: Type u} [HasLin T] {Γ: Ctx T} {v}
+theorem Ctx.var.name {N: Type u} {T: Type v} [HasLin T] {Γ: Ctx N T} {v}
   : Γ.var v -> Γ.name v.name
   | head ⟨H, _, _⟩ _ => H ▸ name.head _ _ _ _
   | tail _ W => name.tail _ (var.name W)
 
-def Ctx.split.left_decompose {T: Type u} [HasLin T] {Γ Δ Ξ: Ctx T}
+def Ctx.split.left_decompose {T: Type u} [HasLin T] {Γ Δ Ξ: Ctx N T}
   : Ctx.split Γ Δ Ξ
-  -> (Δ': Ctx T) × Ctx.ssplit Γ Δ' Ξ × Ctx.wk Δ' Δ
+  -> (Δ': Ctx N T) × Ctx.ssplit Γ Δ' Ξ × Ctx.wk Δ' Δ
   | nil => ⟨[], ssplit.nil, wk.nil⟩
   | left Hl H => let ⟨Δ', HΓ, HΔ⟩ := left_decompose H;
     ⟨_::Δ', ssplit.left Hl HΓ, wk.scons _ HΔ⟩
@@ -238,9 +247,9 @@ def Ctx.split.left_decompose {T: Type u} [HasLin T] {Γ Δ Ξ: Ctx T}
   | dup Hrel Hl Hr H => let ⟨Δ', HΓ, HΔ⟩ := left_decompose H;
     ⟨_::Δ', ssplit.dup Hrel Hl Hr HΓ, wk.scons _ HΔ⟩
 
-def Ctx.split.right_decompose {T: Type u} [HasLin T] {Γ Δ Ξ: Ctx T}
-  : Ctx.split Γ Δ Ξ
-  -> (Ξ': Ctx T) × Ctx.ssplit Γ Δ Ξ' × Ctx.wk Ξ' Ξ
+def Ctx.split.right_decompose {N: Type u} {T: Type v} [HasLin T]
+  {Γ Δ Ξ: Ctx N T}: Ctx.split Γ Δ Ξ
+    -> (Ξ': Ctx N T) × Ctx.ssplit Γ Δ Ξ' × Ctx.wk Ξ' Ξ
   | nil => ⟨[], ssplit.nil, wk.nil⟩
   | left Hl H => let ⟨Ξ', HΓ, HΞ⟩ := right_decompose H;
     ⟨Ξ', ssplit.left Hl HΓ, HΞ⟩
@@ -251,9 +260,9 @@ def Ctx.split.right_decompose {T: Type u} [HasLin T] {Γ Δ Ξ: Ctx T}
   | dup Hrel Hl Hr H => let ⟨Ξ', HΓ, HΞ⟩ := right_decompose H;
     ⟨_::Ξ', ssplit.dup Hrel Hl Hr HΓ, wk.scons _ HΞ⟩
 
-def Ctx.ssplit.distribute_left {T: Type u} [HasLin T] {Γ Γ' Δ Ξ: Ctx T}
-  : Ctx.wk Γ' Γ -> Ctx.ssplit Γ Δ Ξ
-    -> (Δ': Ctx T) × Ctx.ssplit Γ' Δ' Ξ × Ctx.wk Δ' Δ
+def Ctx.ssplit.distribute_left {N: Type u} {T: Type v} [HasLin T]
+  {Γ Γ' Δ Ξ: Ctx N T}: Ctx.wk Γ' Γ -> Ctx.ssplit Γ Δ Ξ
+    -> (Δ': Ctx N T) × Ctx.ssplit Γ' Δ' Ξ × Ctx.wk Δ' Δ
   | wk.nil, nil => ⟨[], ssplit.nil, wk.nil⟩
   | wk.cons Hc W, left Hl S =>
     let ⟨_, HΓ, HΔ⟩ := distribute_left W S;
@@ -274,9 +283,9 @@ def Ctx.ssplit.distribute_left {T: Type u} [HasLin T] {Γ Γ' Δ Ξ: Ctx T}
     let ⟨_, HΓ, HΔ⟩ := distribute_left W S;
     ⟨_, sleft _ HΓ, wk.discard Ha HΔ⟩
 
-def Ctx.ssplit.distribute_right {T: Type u} [HasLin T] {Γ Γ' Δ Ξ: Ctx T}
-  : Ctx.wk Γ' Γ -> Ctx.ssplit Γ Δ Ξ
-    -> (Ξ': Ctx T) × Ctx.ssplit Γ' Δ Ξ' × Ctx.wk Ξ' Ξ
+def Ctx.ssplit.distribute_right {N: Type u} {T: Type v} [HasLin T]
+  {Γ Γ' Δ Ξ: Ctx N T}: Ctx.wk Γ' Γ -> Ctx.ssplit Γ Δ Ξ
+    -> (Ξ': Ctx N T) × Ctx.ssplit Γ' Δ Ξ' × Ctx.wk Ξ' Ξ
   | wk.nil, nil => ⟨[], ssplit.nil, wk.nil⟩
   | wk.cons Hc W, left Hl S =>
     let ⟨_, HΓ, HΞ⟩ := distribute_right W S;
@@ -297,31 +306,31 @@ def Ctx.ssplit.distribute_right {T: Type u} [HasLin T] {Γ Γ' Δ Ξ: Ctx T}
     let ⟨_, HΓ, HΞ⟩ := distribute_right W S;
     ⟨_, sright _ HΓ, wk.discard Ha HΞ⟩
 
-theorem Ctx.wk.length_decreasing {T: Type u} [HasLin T] {Γ Δ: Ctx T} (H: wk Γ Δ)
-  : Δ.length ≤ Γ.length
+theorem Ctx.wk.length_decreasing {T: Type u} [HasLin T] {Γ Δ: Ctx N T}
+  (H: wk Γ Δ): Δ.length ≤ Γ.length
   := Ctx.split.left_length_decreasing H
 
-theorem Ctx.wk.append_false {T: Type u} [HasLin T] {Γ: Ctx T} {A}
+theorem Ctx.wk.append_false {T: Type u} [HasLin T] {Γ: Ctx N T} {A}
   (H: wk Γ (A::Γ)): False
   := have H := H.length_decreasing; by simp_arith at H
 
-theorem Ctx.wk.nil_nil {T: Type u} [HasLin T] {Γ: Ctx T}
+theorem Ctx.wk.nil_nil {T: Type u} [HasLin T] {Γ: Ctx N T}
   : wk [] Γ -> Γ = []
   | nil => rfl
 
 def Ctx.wk.id {T: Type u} [HasLin T]
-  : (Γ: Ctx T) -> Ctx.wk Γ Γ
+  : (Γ: Ctx N T) -> Ctx.wk Γ Γ
   | [] => Ctx.split.nil
   | v::Γ => Ctx.split.left (le_refl v) (id Γ)
 
-instance Ctx.wk.instInhabitedRefl {T: Type u} [HasLin T] {Γ: Ctx T}
-  : Inhabited (Ctx.wk Γ Γ) where
+instance Ctx.wk.instInhabitedRefl {N: Type u} {T: Type v} [HasLin T]
+  {Γ: Ctx N T}: Inhabited (Ctx.wk Γ Γ) where
   default := wk.id Γ
 
-instance Ctx.wk.instSubsingletonRefl {T: Type u} [HasLin T] {Γ: Ctx T}
-  : Subsingleton (Ctx.wk Γ Γ) where
+instance Ctx.wk.instSubsingletonRefl {N: Type u} {T: Type v} [HasLin T]
+  {Γ: Ctx N T}: Subsingleton (Ctx.wk Γ Γ) where
   allEq := let rec allEq
-  : ∀ {Γ: Ctx T} (HΓ: Ctx.wk Γ Γ) (HΓ': Ctx.wk Γ Γ), HΓ = HΓ'
+  : ∀ {Γ: Ctx N T} (HΓ: Ctx.wk Γ Γ) (HΓ': Ctx.wk Γ Γ), HΓ = HΓ'
   | [], nil, nil => rfl
   | _, cons _ HΓ, cons _ HΓ' => congrArg _ (allEq HΓ HΓ')
   | _, discard _ HΓ, _ | _, _, discard _ HΓ => HΓ.append_false.elim
@@ -330,7 +339,7 @@ instance Ctx.wk.instSubsingletonRefl {T: Type u} [HasLin T] {Γ: Ctx T}
 --TODO: subsingleton to nil --> nil is terminal object
 --TODO: subsingleton from nil
 
-def Ctx.wk.comp {T: Type u} [HasLin T] {Γ Δ Ξ: Ctx T}
+def Ctx.wk.comp {N: Type u} {T: Type v}[HasLin T] {Γ Δ Ξ: Ctx N T}
   : Ctx.wk Γ Δ -> Ctx.wk Δ Ξ -> Ctx.wk Γ Ξ
   | nil, nil => nil
   | cons Hl HΓ, cons Hl' HΓ' =>
@@ -340,21 +349,21 @@ def Ctx.wk.comp {T: Type u} [HasLin T] {Γ Δ Ξ: Ctx T}
   | discard Ha HΓ, H =>
     discard Ha (comp HΓ H)
 
-def Ctx.wk.comp_id {T: Type u} [HasLin T] {Γ Δ: Ctx T}
+def Ctx.wk.comp_id {N: Type u} {T: Type v}[HasLin T] {Γ Δ: Ctx N T}
   : (H: Ctx.wk Γ Δ) -> (R: Ctx.wk Δ Δ) -> H.comp R = H
   | nil, nil => rfl
   | cons _ HΓ, cons _ HΓ' => congrArg _ (comp_id HΓ HΓ')
   | discard _ HΓ, HΓ' => congrArg _ (comp_id HΓ HΓ')
   | cons _ _, discard _ HΓ => HΓ.append_false.elim
 
-def Ctx.wk.id_comp {T: Type u} [HasLin T] {Γ Δ: Ctx T}
+def Ctx.wk.id_comp {N: Type u} {T: Type v} [HasLin T] {Γ Δ: Ctx N T}
   : (R: Ctx.wk Γ Γ) -> (H: Ctx.wk Γ Δ) -> R.comp H = H
   | nil, nil => rfl
   | cons _ HΓ, cons _ HΓ' => congrArg _ (id_comp HΓ HΓ')
   | cons _ HΓ, discard _ HΓ' => congrArg _ (id_comp HΓ HΓ')
   | discard _ HΓ, _ => HΓ.append_false.elim
 
-def Ctx.wk.comp_assoc {T: Type u} [HasLin T] {Γ Δ Ξ Θ: Ctx T}
+def Ctx.wk.comp_assoc {N: Type u} {T: Type v} [HasLin T] {Γ Δ Ξ Θ: Ctx N T}
   : (X: Ctx.wk Γ Δ)
   -> (Y: Ctx.wk Δ Ξ)
   -> (Z: Ctx.wk Ξ Θ)
@@ -365,7 +374,7 @@ def Ctx.wk.comp_assoc {T: Type u} [HasLin T] {Γ Δ Ξ Θ: Ctx T}
   | cons _ X, discard _ Y, Z => congrArg _ (comp_assoc X Y Z)
   | discard _ X, Y, Z => congrArg _ (comp_assoc X Y Z)
 
-def Ctx.wk.antisymm {T: Type u} [HasLin T] {Γ Δ: Ctx T}
+def Ctx.wk.antisymm {N: Type u} {T: Type v} [HasLin T] {Γ Δ: Ctx N T}
   : Ctx.wk Γ Δ -> Ctx.wk Δ Γ -> Γ = Δ
   | nil, nil => rfl
   | cons Hl HΓ, cons Hl' HΓ' =>
@@ -380,15 +389,15 @@ def Ctx.wk.antisymm {T: Type u} [HasLin T] {Γ Δ: Ctx T}
     have H := le_trans (Nat.le_step HΓ'.length_decreasing) HΓ.length_decreasing;
     by simp_arith at H
 
-def Ctx.split.right_wk {T: Type u} [HasLin T] {Γ Δ: Ctx T}
+def Ctx.split.right_wk {N: Type u} {T: Type v} [HasLin T] {Γ Δ: Ctx N T}
   : Ctx.split Γ [] Δ → Ctx.wk Γ Δ
   := swap
 
-def Ctx.wk.right_wk {T: Type u} [HasLin T] {Γ Δ: Ctx T}
+def Ctx.wk.right_wk {N: Type u} {T: Type v} [HasLin T] {Γ Δ: Ctx N T}
   : Ctx.wk Γ Δ → Ctx.split Γ [] Δ
   := Ctx.split.swap
 
-def Ctx.wk.equiv_right {T: Type u} [HasLin T] {Γ Δ: Ctx T}
+def Ctx.wk.equiv_right {N: Type u} {T: Type v} [HasLin T] {Γ Δ: Ctx N T}
   : Equiv (Ctx.wk Γ Δ) (Ctx.split Γ [] Δ)
   := Ctx.split.swap_equiv Γ Δ []
 
@@ -397,6 +406,6 @@ def Ctx.wk.equiv_right {T: Type u} [HasLin T] {Γ Δ: Ctx T}
 --   | H, nil => ⟨Δ, H, wk.refl Δ⟩
 --   | _, _ => sorry
 
-def Ctx.var.upgrade {T: Type u} [HasLin T] {Γ: Ctx T} {v v': Var T}
-  (H: Γ.var v) (H': v ≥ v'): Γ.var v'
+def Ctx.var.upgrade {N: Type u} {T: Type v} [HasLin T] {Γ: Ctx N T}
+  {v v': Var N T} (H: Γ.var v) (H': v ≥ v'): Γ.var v'
   := Ctx.wk.comp H (Ctx.wk.cons H' (Ctx.wk.nil))
