Isotope/Syntax/NamedList/LCtx.lean
@@ -2,36 +2,37 @@ import Isotope.Syntax.NamedList.Ctx
 
 namespace NamedList
 
-structure Label (T: Type u) where
-  name: String
-  live: Ctx T
-  param: Var T
+structure Label (N: Type u) (T: Type v) where
+  name: N
+  live: Ctx N T
+  param: Var N T
 
-def Label.subctx {T: Type u} [HasLin T] (Γ: Ctx T) (l: Label T)
+def Label.subctx {N: Type u} {T: Type v} [HasLin T] (Γ: Ctx N T) (l: Label N T)
   := Γ.subctx l.live
 
-structure Label.wk {T: Type u} [HasLin T] (l k: Label T) where
+structure Label.wk {N: Type u} {T: Type v} [HasLin T] (l k: Label N T) where
   name: l.name = k.name
   live: l.live.wk k.live
   param: l.param ≥ k.param
 
-def Label.wk.id {T: Type u} [HasLin T] (l: Label T): l.wk l where
+def Label.wk.id {N: Type u} {T: Type v} [HasLin T] (l: Label N T): l.wk l where
   name := rfl
   live := Ctx.wk.id l.live
   param := le_refl l.param
 
-def Label.wk.comp {T: Type u} [HasLin T] {l k j: Label T}
+def Label.wk.comp {N: Type u} {T: Type v} [HasLin T] {l k j: Label N T}
   (Hlk: l.wk k) (Hkj: k.wk j): l.wk j where
   name := Hlk.name.trans Hkj.name
   live := Ctx.wk.comp Hlk.live Hkj.live
   param := le_trans Hkj.param Hlk.param
 
-abbrev LCtx (T: Type u) := List (Label T)
+abbrev LCtx (N: Type u) (T: Type v) := List (Label N T)
 
-inductive LCtx.lwk {T: Type u} [HasLin T]: LCtx T -> LCtx T -> Type u
+inductive LCtx.lwk {N: Type u} {T: Type v} [HasLin T]
+  : LCtx N T -> LCtx N T -> Type (max u v)
   | nil: lwk [] []
-  | unreached {L K: LCtx T} (l: Label T): lwk L K -> lwk L (l :: K)
-  | cons {L K: LCtx T} {l l': Label T}
+  | unreached {L K: LCtx N T} (l: Label N T): lwk L K -> lwk L (l :: K)
+  | cons {L K: LCtx N T} {l l': Label N T}
     : l.wk l' -> lwk L K  -> lwk (l :: L) (l' :: K)
 
 -- inductive LCtx.sjoin {T: Type u} [HasLin T]: LCtx T -> LCtx T -> Type u
@@ -39,32 +40,33 @@ inductive LCtx.lwk {T: Type u} [HasLin T]: LCtx T -> LCtx T -> Type u
 --   | cons {L K: LCtx T} (l: Label T): sjoin L K -> sjoin (l :: L) (l :: K)
 --   | unreached {L K: LCtx T} (l: Label T): sjoin L K -> sjoin L (l :: K)
 
-def LCtx.lwk.id {T: Type u} [HasLin T]: (L: LCtx T) -> LCtx.lwk L L
+def LCtx.lwk.id {N: Type u} {T: Type v} [HasLin T]: (L: LCtx N T) -> LCtx.lwk L L
   | [] => nil
   | l :: L => cons (Label.wk.id l) (lwk.id L)
 
-def LCtx.lwk.comp {T: Type u} [HasLin T] {L K M: LCtx T}
+def LCtx.lwk.comp {N: Type u} {T: Type v} [HasLin T] {L K M: LCtx N T}
   : LCtx.lwk L K -> LCtx.lwk K M -> LCtx.lwk L M
   | nil, j => j
   | k, unreached l j => unreached l (comp k j)
   | unreached _ j, cons H k => unreached _ (comp j k)
   | cons H j, cons H' k => cons (Label.wk.comp H H') (comp j k)
 
-def LCtx.label {T: Type u} [HasLin T] (L: LCtx T) (l: Label T): Type u
+def LCtx.label {N: Type u} {T: Type v} [HasLin T] (L: LCtx N T) (l: Label N T)
   := LCtx.lwk [l] L
 
-def LCtx.label.wk {T: Type u} [HasLin T] {L: LCtx T} {l k: Label T}
-  (W: l.wk k): L.label k -> L.label l
+def LCtx.label.wk {N: Type u} {T: Type v} [HasLin T] {L: LCtx N T}
+  {l k: Label N T} (W: l.wk k): L.label k -> L.label l
   | lwk.unreached l' j => lwk.unreached l' (wk W j)
   | lwk.cons W' j => lwk.cons (W.comp W') j
 
-inductive LCtx.join {T: Type u} [HasLin T]
-  : (Label T -> Sort v) -> LCtx T -> LCtx T -> LCtx T -> Sort (max (u+1) v)
+inductive LCtx.join {N: Type u} {T: Type v} [HasLin T]
+  : (Label N T -> Sort w) -> LCtx N T -> LCtx N T -> LCtx N T
+    -> Sort (max (max (u+1) (v+1)) w)
   | nil P: join P [] [] []
   | left {P L K J} (l): join P L K J -> join P (l::L) K (l::J)
   | right {P L K J} (r): join P L K J -> join P L (r::K) (r::J)
   | both {P L K J b}: P b -> join P L K J -> join P (b::L) (b::K) (b::J)
   | unreached {P L K J} (l): join P L K J -> join P L K (l::J)
 
-def LCtx.cjoin {T: Type u} [HasLin T] (Γ: Ctx T)
+def LCtx.cjoin {N: Type u} {T: Type v} [HasLin T] (Γ: Ctx N T)
   := LCtx.join (Label.subctx Γ)
